src/gopt/GSimulation.v
@@ -1,0 +1,82 @@
+From sflib Require Import sflib.
+From Paco Require Import paco.
+
+From PromisingLib Require Import Axioms.
+From PromisingLib Require Import Basic.
+From PromisingLib Require Import Loc.
+From PromisingLib Require Import Language.
+
+Require Import Event.
+Require Import View.
+Require Import Cell.
+Require Import Memory.
+Require Import TView.
+Require Import Thread.
+Require Import Configuration.
+Require Import Behavior.
+
+Set Implicit Arguments.
+
+
+Section Simulation.
+  Definition SIM := forall (c1_src c1_tgt: Configuration.t), Prop.
+
+  Inductive _sim (sim: SIM) (c1_src c1_tgt:Configuration.t): Prop :=
+  | _sim_intro
+      (TERMINAL:
+         forall (TERMINAL_TGT: Threads.is_terminal c1_tgt.(Configuration.threads)),
+           <<TERMINAL_SRC: Threads.is_terminal c1_src.(Configuration.threads)>>)
+      (STEP:
+         forall e tid c3_tgt
+           (STEP_TGT: Configuration.step e tid c1_tgt c3_tgt),
+           <<ABORT: Configuration.steps_abort c1_src>> \/
+         exists c2_src c3_src,
+           <<STEPS_SRC: rtc Configuration.tau_step c1_src c2_src>> /\
+           <<STEP_SRC: Configuration.opt_step e tid c2_src c3_src>> /\
+           <<SIM: sim c3_src c3_tgt>>)
+  .
+
+  Lemma _sim_mon: monotone2 _sim.
+  Proof.
+    ii. inv IN. econs; eauto. i.
+    exploit STEP; eauto. i. des; eauto.
+    right. esplits; eauto.
+  Qed.
+  Hint Resolve _sim_mon: paco.
+
+  Definition sim: SIM := paco2 _sim bot2.
+End Simulation.
+Hint Resolve _sim_mon: paco.
+
+
+Lemma sim_adequacy
+      c_src c_tgt
+      (SIM: sim c_src c_tgt):
+  behaviors Configuration.step c_tgt <1= behaviors Configuration.step c_src.
+Proof.
+  i. revert c_src SIM.
+  induction PR; i.
+  - punfold SIM0. inv SIM0. hexploit TERMINAL0; eauto. i. des.
+    econs 1. eauto.
+  - punfold SIM0. inv SIM0. exploit STEP0; eauto. i. des.
+    + inv ABORT. des.
+      eapply rtc_tau_step_behavior; eauto.
+      econs 3; eauto.
+    + inv SIM0; ss.
+      eapply rtc_tau_step_behavior; eauto.
+      inv STEP_SRC. econs 2; eauto.
+  - punfold SIM0. inv SIM0. exploit STEP0; eauto. i. des.
+    + inv ABORT. des.
+      eapply rtc_tau_step_behavior; eauto.
+      econs 3; eauto.
+    + inv SIM0; ss.
+      eapply rtc_tau_step_behavior; eauto.
+      inv STEP_SRC; eauto. econs 3; eauto.
+  - punfold SIM0. inv SIM0. exploit STEP0; eauto. i. des.
+    + inv ABORT. des.
+      eapply rtc_tau_step_behavior; eauto.
+      econs 3; eauto.
+    + inv SIM0; ss.
+      eapply rtc_tau_step_behavior; eauto.
+      inv STEP_SRC; eauto. econs 4; eauto.
+Qed.
